Definition plus propre de l'iterateur exist pour les preuve d'accessibilit�. En vue du talk.

ex_meta1bis.v
@@ -6,60 +6,888 @@ Import ILLVarInt.Tacs. (* only this *)
 Require Import unprove.
 Import FormulaMultiSet. (* and this *)
 Require Import ILL_equiv.
-
+Require Import boolP.
 
 Local Open Scope ILL_scope.
 Local Open Scope Emma.
 Require Import JMeq.
 
-Inductive boolP : Prop := trueP | falseP.
+Generalizable All Variables.
 
-Definition eq_boolP a b := 
-  match a,b with
-    | trueP,trueP => trueP
-    | falseP,falseP => trueP
-    | _,_ => falseP
+Program Fixpoint exist
+  (cont: forall {e1} {f1} (h1: e1 ⊢ f1),boolP)
+  `(h: e ⊢ f) {struct h}: boolP := 
+  match h with
+    | Oplus_R_1 Γ p q h' => cont _ _ h ORP exist cont h'
+    | Oplus_R_2 Γ q p h' => cont _ _ h ORP exist cont h'
+    | Id _ _ p => cont _ _ h
+    | Impl_R Γ p q h' => cont _ _ h ORP exist cont h'
+    | Impl_L Γ Δ Δ' p q r _ _ h' h'0 => cont _ _ h (*ORP exist cont h' *) ORP exist cont h'0
+    | Times_R Γ Δ p q _ _ h' h'0 => cont _ _ h ORP exist cont h' ORP exist cont h'0
+    | Times_L Γ p q r _ h' => cont _ _ h ORP exist cont h'
+    | One_R _ _ => cont _ _ h
+    | One_L Γ p _ h' => cont _ _ h ORP exist cont h'
+    | And_R Γ p q h' h'0 => cont _ _ h ORP exist cont h' ORP exist cont h'0
+    | And_L_1 Γ p q r _ h' => cont _ _ h ORP exist cont h'
+    | And_L_2 Γ p q r _ h' => cont _ _ h ORP exist cont h'
+    | Oplus_L Γ p q r _ h' h'0 => cont _ _ h ORP exist cont h' ORP exist cont h'0
+    | T_ Γ => cont _ _ h
+    | Zero_ Γ p h' => cont _ _ h
+    | Bang_D Γ p q _ h' => cont _ _ h ORP exist cont h'
+    | Bang_C Γ p q _ h' => cont _ _ h ORP exist cont h'
+    | Bang_W Γ p q _ h' => cont _ _ h ORP exist cont h'
   end.
 
-  Infix "?=" := eq_boolP (at level 80).
 
-  Definition orP a b :=
-    match a with
-      | trueP => trueP
-      | falseP => b
-    end.
-
-
-  Definition andP a b :=
-    match a with
-      | falseP => falseP
-      | trueP => b
-    end.
-
-Infix "ORP" := orP (at level 70).
-Infix "ANDP" := andP (at level 70).
-
-
-Program Fixpoint check
+Program Fixpoint for_all
   (cont: forall (e1:env) (f1:formula) (h1: e1 ⊢ f1),boolP)
-  (e:env) (f:formula) (h: e ⊢ f) {struct h}: boolP := 
-match h with
-  | Oplus_R_1 Γ p q x => (cont _ _ h) ORP (check cont _ _ x)
-  | Oplus_R_2 Γ q p x => (cont _ _ h) ORP (check cont _ _ x)
-  | Id _ _ p => (cont _ _ h)
-  | Impl_R Γ p q x => check cont _ _ x
-  | Impl_L Γ Δ Δ' p q r _ _ x x0 => check cont _ _ x
-  | Times_R Γ Δ p q _ _ x x0 => if check cont _ _ x then trueP else check cont _ _ x0
-  | Times_L Γ p q r _ x => check cont _ _ x
-  | One_R _ _ => falseP
-  | One_L Γ p _ x => check cont _ _ x
-  | And_R Γ p q x x0 => if check cont _ _ x then trueP else check cont _ _ x0
-  | And_L_1 Γ p q r _ x => check cont _ _ x
-  | And_L_2 Γ p q r _ x => check cont _ _ x
-  | Oplus_L Γ p q r _ x x0 => if check cont _ _ x then trueP else check cont _ _ x0
-  | T_ Γ => falseP
-  | Zero_ Γ p x => falseP
-  | Bang_D Γ p q _ x => check cont _ _ x
-  | Bang_C Γ p q _ x => check cont _ _ x
-  | Bang_W Γ p q _ x => check cont _ _ x
-end.
+  `(h: e ⊢ f) {struct h}: boolP := 
+  match h with
+    | Oplus_R_1 Γ p q h' => cont _ _ h ORP for_all cont h'
+    | Oplus_R_2 Γ q p h' => cont _ _ h ORP for_all cont h'
+    | Id _ _ p => cont _ _ h
+    | Impl_R Γ p q h' => cont _ _ h ORP for_all cont h'
+    | Impl_L Γ Δ Δ' p q r _ _ h' h'0 => cont _ _ h ORP for_all cont h'
+    | Times_R Γ Δ p q _ _ h' h'0 => cont _ _ h ORP (for_all cont h' ANDP for_all cont h'0)
+    | Times_L Γ p q r _ h' => cont _ _ h ORP for_all cont h'
+    | One_R _ _ => cont _ _ h
+    | One_L Γ p _ h' => cont _ _ h ORP for_all cont h'
+    | And_R Γ p q h' h'0 => cont _ _ h ORP (for_all cont h' ANDP for_all cont h'0)
+    | And_L_1 Γ p q r _ h' => cont _ _ h ORP for_all cont h'
+    | And_L_2 Γ p q r _ h' => cont _ _ h ORP for_all cont h'
+    | Oplus_L Γ p q r _ h' h'0 => cont _ _ h ORP (for_all cont h' ANDP for_all cont h'0)
+    | T_ Γ => cont _ _ h
+    | Zero_ Γ p h' => cont _ _ h
+    | Bang_D Γ p q _ h' => cont _ _ h ORP for_all cont h'
+    | Bang_C Γ p q _ h' => cont _ _ h ORP for_all cont h'
+    | Bang_W Γ p q _ h' => cont _ _ h ORP for_all cont h'
+  end.
+
+Definition eq_formula_boolP e f := 
+  if FormulaOrdered.eq_dec e f then trueP else falseP.
+
+Infix "?=?" := eq_formula_boolP (at level 60).
+
+Definition choices_between_A_and_M e f `{h: e ⊢ f} := 
+  match h with
+    | Oplus_L Γ p q r _ x x0 => p ?=? A ANDP q ?=? M
+    | _ => falseP
+  end.
+
+Definition choices_between_S_and_R e f `{h: e ⊢ f} := 
+  match h with
+    | Oplus_L Γ p q r _ x x0 => p ?=? S ANDP q ?=? R
+    | _ => falseP
+  end.
+
+Definition right_choices_between_A_and_M e f `{h: e ⊢ f} := 
+  match h with
+    | Oplus_R_1 Γ p q x => p?=?A ANDP q?=?M
+    | Oplus_R_2 Γ p q x => p?=?A ANDP q?=?M
+    | _ => falseP
+  end.
+
+Definition yes e f `{h: e ⊢ f} := trueP.
+
+Definition essai e f `{h: e ⊢ f} := 
+  match h with
+    | Oplus_L Γ p q r _ x x0 => p ?=? (G ⊸ 1) ANDP q ?=? (G ⊸ S)
+    | _ => falseP
+  end.
+
+Definition essai2 e f `{h: e ⊢ f} := 
+  match h with
+    | And_L_1 Γ p q r _ x => p ?=? B
+    | _ => falseP
+  end.
+
+Eval vm_compute in (exist essai2 originelle).
+Eval vm_compute in (exist choices_between_A_and_M originelle).
+Eval vm_compute in (exist choices_between_S_and_R originelle).
+Eval vm_compute in (exist right_choices_between_A_and_M originelle).
+Eval vm_compute in (exist right_choices_between_A_and_M simpl_ex).
+
+Lemma simple: { G, ((B⊸S)&(B⊸R))&1,(G⊸B)⊕(G⊸S)} ⊢ S⊕R.
+Proof with try solve [ apply Id;reflexivity | prove_multiset_eq].
+  oplus_l (G⊸B) (G⊸S).
+  weak_impl_l G B...
+  and_l_1 ((B ⊸ S) & (B ⊸ R)) 1.
+
+  and_l_1 (B ⊸ S) (B ⊸ R).
+  weak_impl_l B S...
+  apply Oplus_R_1...
+
+(* 
+  and_l_2 (B ⊸ S) (B ⊸ R).
+  weak_impl_l B R...
+  apply Oplus_R_2...
+ *)
+
+  weak_impl_l G S...
+  and_l_2 ((B ⊸ S) & (B ⊸ R)) 1.
+  one_l.
+  apply Oplus_R_1...
+Defined.
+
+Eval vm_compute in (exist choices_between_A_and_M simple).
+
+
+Lemma orP_right : ∀ (a b c:boolP) , a = b -> a ORP c = (b ORP c).
+Proof.
+  intros a b c H.  
+  rewrite H.
+  destruct b;simpl;auto.
+Qed.
+  
+Class f_comp (f:(∀ `(h:e1 ⊢ f1), boolP)) := {
+  fcomp : (∀ Γ Γ' φ (h1:Γ⊢φ) (h2:Γ'⊢φ), Proof_eq.eq h1 h2 -> f h1 = f h2)
+}.
+
+
+
+Definition f_comp_eq `(f1:f_comp f) `(f2:f_comp f) := True.
+
+Lemma f_comp_eq_refl: forall `(f1:f_comp f), f_comp_eq f1 f1.
+  reflexivity.
+Qed.
+
+Lemma f_comp_eq_sym: forall `(f1:f_comp f) `(f2:f_comp f), f_comp_eq f1 f2 -> f_comp_eq f2 f1.
+  trivial.
+Qed.
+
+Lemma f_comp_eq_trans: forall `(f1:f_comp f) `(f2:f_comp f) `(f3:f_comp f), f_comp_eq f1 f2 -> f_comp_eq f2 f3 -> f_comp_eq f1 f3.
+  trivial.
+Qed.
+
+Require Import Setoid.
+
+  
+Add Parametric Relation {f}: (f_comp f) f_comp_eq
+  reflexivity proved by f_comp_eq_refl
+  symmetry proved by f_comp_eq_sym
+    transitivity proved by f_comp_eq_trans
+      as f_com_eq_R.
+
+Lemma exists_AtheseA_on_formula_proof_eq_compat : 
+  ∀ `(h:f_comp f),
+  ∀ Γ Γ' φ (h1:Γ⊢φ) (h2:Γ'⊢φ),  Proof_eq.eq h1 h2 -> exist f h1 = exist f h2.
+Proof.
+  intros f H Γ Γ' φ h1 h2 H0.
+  induction H0;simpl;try complete (
+    try rewrite IHeq; try rewrite IHeq1;try rewrite IHeq2;
+      repeat apply orP_right;apply H;auto;subst;auto;
+          try setoid_rewrite (H Γ1 Γ2);eauto;try constructor;auto ).
+Qed.
+
+
+Lemma exists_AtheseA_on_formula_proof_eq_pre_morph_compat : 
+  ∀ `(h:f_comp f),
+  (∀ Γ Γ' φ (h1:Γ⊢φ) (h2:Γ'⊢φ), Proof_eq.eq h1 h2 -> f _ _ h1 = f _ _ h2) -> 
+  ∀ Γ Γ' φ (h1:Γ⊢φ) (h2:Γ==Γ'), 
+  exist f h1
+  = exist f (ILL_proof_pre_morph φ Γ Γ' h2 h1).
+Proof.
+  intros f h H Γ Γ' φ h1 h2.
+  apply exists_AtheseA_on_formula_proof_eq_compat.
+  assumption.
+  apply Proof_eq.sym;apply Proof_eq.eq_pre_morph.
+Qed.
+
+
+  
+Definition all_proofsof `(h:f_comp f) e gamma :=
+  (forall (p:e⊢gamma), exist f p =trueP).
+
+Definition no_proof_for env gamma := (forall (p:env⊢gamma), False).
+Hint Unfold all_proofsof no_proof_for : proof.
+
+Lemma all_proofsof_pre_morph : forall φ Γ Γ' `(h:f_comp f),  
+  all_proofsof h Γ φ -> eq_bool Γ Γ' = true -> all_proofsof h Γ' φ.
+Proof.
+  unfold all_proofsof.
+  intros φ Γ Γ' f h H Heq p.
+  apply eq_bool_correct in Heq.
+  assert (h':exists p': Γ⊢φ, Proof_eq.eq p p').
+    symmetry in Heq; exists (ILL_proof_pre_morph _ _ _ Heq p).
+    apply Proof_eq.sym;apply Proof_eq.eq_pre_morph.
+      destruct h' as [p' h'].
+      setoid_rewrite (exists_AtheseA_on_formula_proof_eq_compat); eauto.
+Qed.
+Hint Resolve all_proofsof_pre_morph : proof.
+
+
+Lemma all_proofsof_pre_morph' : 
+  forall φ Γ Γ' `(h:f_comp f),
+    all_proofsof h Γ φ -> eq_bool Γ Γ' = true -> 
+    forall (p:Γ'⊢φ), exist f p =trueP.
+Proof.
+  intros φ Γ Γ' f h H H0 p.
+  eapply all_proofsof_pre_morph;eauto.
+Qed.
+Hint Resolve all_proofsof_pre_morph' : proof.
+Hint Rewrite all_proofsof_pre_morph' : proof.
+
+Add Parametric Morphism `(h:f_comp f):
+  (all_proofsof h)
+  with signature (eq ==> Logic.eq ==> iff)
+    as all_proof_of_morph.
+Proof.
+  intros x y H φ.
+  split;intros;eauto;
+    eapply all_proofsof_pre_morph;eauto;try apply eq_bool_complete;try assumption;try symmetry;try assumption.
+Qed.
+
+Hint Extern 0 ( _ ==  _ ) => apply eq_bool_correct;vm_compute;reflexivity : proof.
+
+
+Ltac clean p := 
+  try complete eauto 2 with proof;
+    (dependent simple inversion p||inversion p);clear p;subst;try discriminate;simpl.
+
+
+Ltac decompose_add := 
+    repeat (match goal with 
+            | H : _ ∈ (_ :: _) |- _  => 
+              destruct (mem_destruct _ _ _ H);clear H
+            | H : _ ∈ ∅ |- _ => 
+              rewrite empty_no_mem in H;discriminate
+            | H : ILLVarInt.MILL.eq _ _ |- _ => apply eq_is_eq in H;subst
+          end).
+
+Ltac var_not_in_env_tac_simple n' H := 
+elim unusable_var_in_env with (n:=n') (1:=H);
+[
+  vm_compute;reflexivity |
+  vm_compute;reflexivity |
+  vm_compute;reflexivity |
+  vm_compute;reflexivity |
+    intros;decompose_add;simpl in *;repeat split;try discriminate;reflexivity
+]
+.
+
+Ltac var_not_in_env_tac_aux H env := 
+  match env with 
+    | Proposition ?n::?env' =>
+      (complete (var_not_in_env_tac_simple n H)) || 
+        var_not_in_env_tac_aux H env'
+    | _ :: ?env' =>  var_not_in_env_tac_aux H env'
+  end.
+
+Ltac var_not_in_env_tac H := 
+  match type of H with 
+    | ?env ⊢ _ => 
+      var_not_in_env_tac_aux H env
+  end.
+Ltac is_var_env gamma := 
+  match gamma with 
+    | empty => fail 1
+    | _ :: _ => fail 1
+    | _ \ _ => fail 1
+    | _ ∪ _ => fail 1
+    | _ => idtac
+  end.
+
+(*Ltac tutu := 
+  simpl;try reflexivity;
+    try discriminate;
+      try complete auto with proof;
+        (* try autorewrite with proof; *)
+          match goal with
+            | H : ?t == _ |- _ => 
+              is_var_env t;
+              match goal with 
+                | H': context [t] |- _ => 
+                  match H' with 
+                    | H => fail 1
+                    | _ => fail 2
+                  end
+                | _ => clear H
+              end
+          
+            | H : ?t = ?t |- _ => clear H
+            | H : ?t == ?t |- _ => clear H
+            | H:_ :: _ == _ ∪ _ |- _ => 
+              symmetry in H
+            | H: _ ∪ _ == _ :: _ |- _ => 
+              let delta := fresh "Δ" in
+                let h1 := fresh "H" in 
+                  let h2 := fresh "H" in 
+                    destruct (union_decompose _ _ _ _ H) 
+                      as [[delta [h1 h2]]|[delta [h1 h2]]];clear H
+            | H: empty == _ ∪ _ |- _ => 
+              symmetry in H
+            | H: _ ∪ _ == empty |- _ => 
+              let h1 := fresh "H" in 
+                let h2 := fresh "H" in 
+                  destruct (union_empty_decompose _ _  H) as [h1 h2];
+                    clear H
+         | H: ILLVarInt.MILL.eq _ _ |- _ => apply eq_is_eq in H; try (injection H;clear H;intros;subst)
+
+            | H: _ ∈ _ |- _ => complete (vm_compute in H;discriminate)
+            | H: _ ∈ (add _ _) |- _ =>   
+              destruct (mem_destruct _ _ _ H);clear H
+            | H : ?s == ?t |- _ => 
+              (complete (apply eq_bool_complete in H;vm_compute in H;
+                discriminate))|| (progress repeat (rewrite H in * ))
+            | H: context C [ remove ?f ?env ] |- _ => 
+              match env with 
+                context C' [ add f ?env' ] => 
+                let e := context C' [ env' ] in 
+                  setoid_replace (remove f env) with e in H by (apply eq_bool_correct;vm_compute;reflexivity)
+              end
+            | H:(?x ⊸ ?y) = _  |- _ => 
+              try discriminate H;injection H;clear H;intros;subst
+            | H: (_ ⊕ _) = _  |- _ => 
+              try discriminate H;injection H;clear H;intros;subst
+            | H:(_ ⊗ _) = _ |- _  => 
+              try discriminate H;injection H;clear H;intros;subst
+            | H: _  & _ = _  |- _  => 
+              try discriminate H;injection H;clear H;intros;subst
+            | H: _ = (?x ⊸ ?y) |- _ => 
+              try discriminate H;injection H;clear H;intros;subst
+            | H: _ = (_ ⊕ _) |- _ => 
+              try discriminate H;injection H;clear H;intros;subst
+            | H: _ = (_ ⊗ _) |- _  => 
+              try discriminate H;injection H;clear H;intros;subst
+            | H: _ = _  & _ |- _  => 
+              try discriminate H;injection H;clear H;intros;subst
+            | H: ?delta ⊢ _, H' : ?delta == ∅ |- _ => 
+              apply False_ind;rewrite H' in H;clear H';clean H;repeat tutu
+            | H: ?env⊢?g |- _ =>
+(*              try complete var_not_in_env_tac H; *)
+                match env with 
+                  | context C' [?env' \ ?f] => 
+                    match env' with 
+                      | context C [add f ?env''] => 
+                        let e' := context C [ env'' ] in 
+                          let e := context C' [ e' ] in 
+                            assert (heq: e == env) by (apply eq_bool_correct;vm_compute;reflexivity);
+                              symmetry in heq;
+                                let h := fresh "H" in 
+                                  let i' := fresh "i" in 
+                                    assert (h:(exists i':ILL_proof e g, Proof_eq.eq H i')) by (exists (ILL_proof_pre_morph _ _ _ heq H);
+                                      apply Proof_eq.sym;
+                                    apply Proof_eq.eq_pre_morph);
+          destruct h as [i' h];
+            rewrite exists_AtheseA_on_formula_proof_eq_compat with (h2:=i') (2:=h);
+              clear H h heq
+end
+end
+            | H: ?t == ?t', i: ?env⊢?f |- _ => 
+              match env with 
+                | context [ t ] => 
+                  let f_env := 
+                    match eval pattern t in env with
+                      | ?f _ => f
+                    end
+                    in
+                    let env'0 := constr:(f_env t')  in 
+                      let env' := eval cbv beta iota in env'0 in 
+                        let h := fresh "H" in 
+                          let i' := fresh "i" in 
+                            let heq := fresh "heq" in 
+                              assert (h:exists i': env'⊢f, Proof_eq.eq i i');[
+                                assert (heq:env'==env) by (rewrite H;reflexivity);
+                                  symmetry in heq;
+                                    exists (ILL_proof_pre_morph _ _ _ heq i);
+                                      apply Proof_eq.sym;apply Proof_eq.eq_pre_morph
+|
+  destruct h as [i' h];
+    rewrite exists_AtheseA_on_formula_proof_eq_compat with (h2:=i') (2:=h);clear i h;try (rewrite H in *;clear H)
+]
+end
+
+          end.
+
+
+Ltac finish := 
+  simpl;try reflexivity;
+    try discriminate;
+    try complete auto with proof;
+    try autorewrite with proof;
+      try complete (apply False_ind;auto with proof);
+      match goal with 
+        | |- (if ?e then trueP else trueP ) = trueP => 
+          case e;reflexivity
+        | H: ?env⊢?g |- _ => complete var_not_in_env_tac H
+        | i:?e⊢Proposition ?n' |- _ => 
+          elim var_in_env with (n:=n') (3:=i);vm_compute;reflexivity
+      end.
+*)
+
+
+Ltac finish := 
+  simpl;try reflexivity;
+    try discriminate;
+    try complete auto with proof;
+    try autorewrite with proof;
+      try complete (apply False_ind;auto with proof);
+      match goal with 
+        |- (if ?e then trueP else trueP ) = trueP => 
+          case e;reflexivity
+        | i:?e⊢Proposition ?n' |- _ => 
+          elim var_in_env with (n:=n') (3:=i);vm_compute;reflexivity
+        | H: ?env⊢?g |- _ =>
+          complete var_not_in_env_tac H
+        | H : ?s == ?t |- _ => 
+          (complete (apply eq_bool_complete in H;vm_compute in H;
+            discriminate))|| (progress repeat (rewrite H in * ))
+      end.
+
+Ltac decomp := 
+  simpl;try reflexivity;
+    try discriminate;
+      (* try complete auto with proof; *)
+        (* try autorewrite with proof; *)
+          match goal with
+            | H : ?t = ?t |- _ => clear H
+            | H : ?t == ?t |- _ => clear H
+            | H:_ :: _ == _ ∪ _ |- _ => 
+              symmetry in H
+            | H: _ ∪ _ == _ :: _ |- _ => 
+              let delta := fresh "Δ" in
+                let h1 := fresh "H" in 
+                  let h2 := fresh "H" in 
+                    destruct (union_decompose _ _ _ _ H) 
+                      as [[delta [h1 h2]]|[delta [h1 h2]]];clear H
+            | H: empty == _ ∪ _ |- _ => 
+              symmetry in H
+            | H: _ ∪ _ == empty |- _ => 
+              let h1 := fresh "H" in 
+                let h2 := fresh "H" in 
+                  destruct (union_empty_decompose _ _  H) as [h1 h2];
+                    clear H
+            | H : ?t == _ |- _ => 
+              is_var_env t;
+              match goal with 
+                | H': context [t] |- _ => 
+                  match H' with 
+                    | H => fail 1
+                    | _ => fail 2
+                  end
+                | _ => clear H
+              end
+            | H: ILLVarInt.MILL.eq _ _ |- _ => apply eq_is_eq in H; try (injection H;clear H;intros;subst)
+
+            | H: _ ∈ _ |- _ => complete (vm_compute in H;discriminate)
+            | H: _ ∈ (add _ _) |- _ =>   
+              destruct (mem_destruct _ _ _ H);clear H
+            (* | H : ?s == ?t |- _ =>  *)
+            (*   (complete (apply eq_bool_complete in H;vm_compute in H; *)
+            (*     discriminate))|| (progress repeat (rewrite H in * )) *)
+            | H : ?s == ?t |- _ => 
+              (progress repeat (rewrite H in * ))
+            | H: context C [ remove ?f ?env ] |- _ => 
+              match env with 
+                context C' [ add f ?env' ] => 
+                let e := context C' [ env' ] in 
+                  setoid_replace (remove f env) with e in H by (apply eq_bool_correct;vm_compute;reflexivity)
+              end
+            | H:(?x ⊸ ?y) = _  |- _ => 
+              try discriminate H;injection H;clear H;intros;subst
+            | H: (_ ⊕ _) = _  |- _ => 
+              try discriminate H;injection H;clear H;intros;subst
+            | H:(_ ⊗ _) = _ |- _  => 
+              try discriminate H;injection H;clear H;intros;subst
+            | H: _  & _ = _  |- _  => 
+              try discriminate H;injection H;clear H;intros;subst
+            | H: _ = (?x ⊸ ?y) |- _ => 
+              try discriminate H;injection H;clear H;intros;subst
+            | H: _ = (_ ⊕ _) |- _ => 
+              try discriminate H;injection H;clear H;intros;subst
+            | H: _ = (_ ⊗ _) |- _  => 
+              try discriminate H;injection H;clear H;intros;subst
+            | H: _ = _  & _ |- _  => 
+              try discriminate H;injection H;clear H;intros;subst
+            | H: ?delta ⊢ _, H' : ?delta == ∅ |- _ => 
+              apply False_ind;rewrite H' in H;clear - H;clean H;finish
+            | H: ?env⊢?g |- _ =>
+              (* try complete var_not_in_env_tac H;  *)
+                match env with 
+                  | context C' [?env' \ ?f] => 
+                    match env' with 
+                      | context C [add f ?env''] => 
+                        let e' := context C [ env'' ] in 
+                          let e := context C' [ e' ] in 
+                            assert (heq: e == env) by (apply eq_bool_correct;vm_compute;reflexivity);
+                              symmetry in heq;
+                                let h := fresh "H" in 
+                                  let i' := fresh "i" in 
+                                    assert (h:(exists i':ILL_proof e g, Proof_eq.eq H i')) by (exists (ILL_proof_pre_morph _ _ _ heq H);
+                                      apply Proof_eq.sym;
+                                    apply Proof_eq.eq_pre_morph);
+          destruct h as [i' h];
+            rewrite exists_AtheseA_on_formula_proof_eq_compat with (h2:=i') (2:=h);
+              clear H h heq
+end
+end
+            | H: ?t == ?t', i: ?env⊢?f |- _ => 
+              match env with 
+                | context [ t ] => 
+                  let f_env := 
+                    match eval pattern t in env with
+                      | ?f _ => f
+                    end
+                    in
+                    let env'0 := constr:(f_env t')  in 
+                      let env' := eval cbv beta iota in env'0 in 
+                        let h := fresh "H" in 
+                          let i' := fresh "i" in 
+                            let heq := fresh "heq" in 
+                              assert (h:exists i': env'⊢f, Proof_eq.eq i i');[
+                                assert (heq:env'==env) by (rewrite H;reflexivity);
+                                  symmetry in heq;
+                                    exists (ILL_proof_pre_morph _ _ _ heq i);
+                                      apply Proof_eq.sym;apply Proof_eq.eq_pre_morph
+|
+  destruct h as [i' h];
+    rewrite exists_AtheseA_on_formula_proof_eq_compat with (h2:=i') (2:=h);clear i h;try (rewrite H in *;clear H)
+]
+end
+
+          end.
+
+
+
+Ltac one_step p :=   clean p; (repeat decomp);try finish;auto with proof;eauto 3 with proof.
+
+Ltac unusable_implies_tac n' f H := 
+  apply unusable_implies with (1:=H) (n:=n') (φ:=f);
+    [
+      vm_compute;reflexivity |
+        vm_compute;reflexivity |
+          vm_compute;reflexivity |
+            intros;decompose_add;repeat split;simpl in *;try discriminate;reflexivity].
+
+Ltac unusable_var_strong_tac n1 n2 H :=
+  apply unusable_var_in_env_strong with (1:=H) (n:=n1);[
+  vm_compute;reflexivity|
+  vm_compute;reflexivity|
+  vm_compute;reflexivity|
+  vm_compute;reflexivity|
+  intros;decompose_add;simpl in *;  repeat split;try discriminate;try reflexivity;auto;
+  intros _;right;
+  exists n2;
+    split;[((left;reflexivity)||(right;reflexivity))|split;[
+      intros;decompose_add;simpl;reflexivity|vm_compute;reflexivity]]].
+
+
+Section ex_meta1.
+
+  Definition right_choices_between_S_and_R e f `{h: e ⊢ f} := 
+    match h with
+      | Oplus_R_1 Γ p q x => p?=?S ANDP q?=?R
+      | Oplus_R_2 Γ p q x => p?=?S ANDP q?=?R
+      | _ => falseP
+    end.
+
+  Instance checkSR :f_comp right_choices_between_S_and_R.
+  Proof.
+    constructor.
+    intros Γ Γ' φ h1 h2 H.
+    induction H;simpl;try reflexivity.
+  Defined.
+
+  Hint Immediate checkSR:proof.
+
+  Definition all_proofs_of := all_proofsof checkSR.
+
+
+
+Lemma aux3 : all_proofs_of ({S}) (S ⊕ R).
+Proof.
+  intros p ; one_step p.
+Qed.
+
+Lemma aux4 : no_proof_for ({G ⊸ S, B ⊸ S, G}) (S ⊕ R).
+Proof.
+  intros p.
+  unusable_implies_tac 4 S p.
+Qed.
+Lemma aux4' : no_proof_for ({B ⊸ S,G ⊸ S,  G}) (S ⊕ R).
+Proof.
+  intros p.
+  unusable_implies_tac 4 S p.
+Qed.
+
+Lemma aux6 : no_proof_for ({G, (G ⊸ B) ⊕ (G ⊸ S)}) B.
+Proof.
+  intros p. one_step p.
+Qed.
+
+Lemma aux2 : all_proofs_of ({B ⊸ S, G, (G ⊸ B) ⊕ (G ⊸ S)}) (S ⊕ R).
+  intros p ; one_step p.
+  exfalso.
+  apply aux6.
+  assumption.
+  apply False_ind.
+  apply aux4.
+  assumption.
+Qed.
+
+
+Lemma aux8 : ∀ x, no_proof_for ({B ⊸ R, G}) (Proposition x).
+Proof.
+  intros H p.
+  unusable_implies_tac 4 R p.
+Qed.
+
+Lemma aux9 : no_proof_for ({S,B ⊸ R}) (S ⊕ R).
+Proof.
+  intros p.
+  unusable_implies_tac 4 R p.
+Qed.
+
+
+Lemma aux9' : no_proof_for ({B ⊸ R,S}) (S ⊕ R).
+Proof.
+  intros p.
+  unusable_implies_tac 4 R p.
+Qed.
+
+Lemma aux9's : no_proof_for ({B ⊸ R,S}) S.
+Proof.
+  intros p.
+  unusable_implies_tac 4 R p.
+Qed.
+Lemma aux10 : ∀ x,no_proof_for ({G ⊸ S, B ⊸ R, G}) (Proposition x).
+Proof.
+  intros H p.
+  unusable_implies_tac 4 R p.
+Qed.
+
+Lemma aux11 : no_proof_for ({B ⊸ R, G, (G ⊸ B) ⊕ (G ⊸ S)}) S.
+Proof.
+  intros p; one_step p.
+Qed.
+Lemma aux12 : no_proof_for ({B ⊸ R, G, (G ⊸ B) ⊕ (G ⊸ S)}) R.
+Proof.
+  intros p; one_step p.
+  apply aux6;assumption.
+  eapply aux10;eassumption.
+Qed.
+
+
+Lemma aux7 : no_proof_for ({G ⊸ S, B ⊸ R, G}) (S ⊕ R).
+Proof.
+  intro p. one_step p.
+  eapply aux8;eassumption.
+  eapply aux9. eassumption.
+  eapply aux10. eassumption.
+  eapply aux10. eassumption.
+Qed.
+
+
+Lemma aux5 : no_proof_for ({B ⊸ R, G, (G ⊸ B) ⊕ (G ⊸ S)}) (S ⊕ R).
+Proof.
+  intros p; one_step p.
+  apply False_ind.
+  apply aux6.
+  assumption.
+  apply aux7;assumption.
+  apply aux11;assumption.
+  apply aux12;assumption.
+Qed.
+
+
+Lemma aux13 : no_proof_for ({B ⊸ R, G, (G ⊸ B) ⊕ (G ⊸ S)}) (S ⊕ R).
+  intros p; one_step p.
+  apply aux6. assumption.
+  apply aux7. assumption.
+  apply aux11. assumption.
+  apply aux12. assumption.
+Qed.
+
+Lemma aux16 :no_proof_for ({B ⊸ S, G}) G.
+  intro p. unusable_implies_tac 4 S p.
+Qed.
+
+Lemma aux15 :no_proof_for ({(B ⊸ S) & (B ⊸ R), G}) G.
+  intro p. one_step p.
+  apply aux16. assumption.
+  eapply aux8;eassumption.
+Qed.
+
+Lemma aux18 : no_proof_for ({B ⊸ S, S}) (S ⊕ R).
+  intro p. unusable_implies_tac 4 S p.
+Qed.
+
+Lemma aux18s :no_proof_for ({B ⊸ S, S}) (S).
+  intro p. unusable_implies_tac 4 S p.
+Qed.
+
+Lemma aux19 : no_proof_for ({S, (B ⊸ S) & (B ⊸ R)}) S.
+  intro p. one_step p.
+
+
+  apply aux18s. assumption.
+  apply aux9's. assumption.
+Qed.
+
+Lemma aux17 : no_proof_for ({S, (B ⊸ S) & (B ⊸ R)}) (S ⊕ R).
+  intro p. one_step p.
+  apply aux18. assumption.
+  apply aux9'. assumption.
+  apply aux19. assumption.
+Qed.
+Lemma aux10' : no_proof_for ({B ⊸ R,G ⊸ S, G}) (S ⊕ R).
+Proof.
+  intros p.
+  unusable_implies_tac 4 R p.
+Qed.
+Lemma aux10's : no_proof_for ({B ⊸ R,G ⊸ S, G}) S.
+Proof.
+  intros p.
+  unusable_implies_tac 4 R p.
+Qed.
+Lemma aux21 : no_proof_for ({(B ⊸ S) & (B ⊸ R), G}) G.
+  intro p. one_step p.
+  apply aux16. assumption.
+  eapply aux8. eassumption.
+Qed.
+Lemma aux15s : no_proof_for ({S,(B ⊸ S) & (B ⊸ R)}) S.
+  intro p. one_step p.
+
+  apply aux18s. assumption.
+  eapply aux9's;eassumption.
+Qed.
+Lemma aux4's : no_proof_for ({B ⊸ S,G ⊸ S,  G}) S.
+Proof.
+  intros p.
+  unusable_implies_tac 4 S p.
+Qed.
+
+Lemma aux20 : no_proof_for ({G ⊸ S, (B ⊸ S) & (B ⊸ R), G}) S.
+  intro p. one_step p.
+  apply aux21. assumption.
+  apply aux15s. assumption.
+  apply aux4's. assumption.
+  apply aux10's. assumption.
+Qed.
+Lemma aux10'r : no_proof_for ({B ⊸ R,G ⊸ S, G}) R.
+Proof.
+  intros p.
+  unusable_implies_tac 4 R p.
+Qed.
+Lemma aux22 : no_proof_for ({G ⊸ S, (B ⊸ S) & (B ⊸ R), G}) R.
+  intro p. one_step p.
+
+  apply aux10'r. assumption.
+Qed.
+Lemma aux14 : no_proof_for ({G ⊸ S, (B ⊸ S) & (B ⊸ R), G}) (S ⊕ R).
+  intro p. one_step p.
+  apply  aux15. assumption.
+  apply aux17. assumption.
+  apply aux4'. assumption.
+  apply aux10'. assumption.
+  apply aux20. assumption.
+  apply aux22. assumption.
+Qed.
+
+
+
+Hint Resolve aux3 aux4 aux4' aux2 aux6 aux8 aux9 aux9' aux9's
+  aux10 aux11 aux12 aux7 aux5 aux13 aux16 aux15
+  aux18 aux18s aux19 aux17 aux10' aux10's aux21
+  aux15s aux4's aux20 aux10'r aux22 aux14:proof.
+
+
+Lemma aux23 : no_proof_for ({(B ⊸ S) & (B ⊸ R), G, (G ⊸ B) ⊕ (G ⊸ S)}) R.
+  intro p. one_step p.
+Qed.
+
+Lemma aux25 : no_proof_for ({G ⊸ B, G}) (S⊕R).
+Proof.
+  intros p. one_step p.
+Qed.
+Lemma aux6'' : no_proof_for ({G, (G ⊸ B) ⊕ (G ⊸ S)}) (S).
+Proof.
+  intros p. one_step p.
+Qed.
+Lemma aux6' : no_proof_for ({G, (G ⊸ B) ⊕ (G ⊸ S)}) (S⊕R).
+Proof.
+  intros p. one_step p.
+  
+  apply aux25. assumption.
+
+  apply aux6''. assumption.
+Qed.
+Lemma aux26 : no_proof_for ({G ⊸ B, 1, G}) (S ⊕ R).
+  intro p. one_step p.
+  apply aux25;assumption.
+Qed.
+Lemma aux24s : no_proof_for ({1, G, (G ⊸ B) ⊕ (G ⊸ S)}) S.
+  intro p. one_step p.
+  apply aux6''. assumption.
+Qed.
+
+Lemma aux24 : no_proof_for ({1, G, (G ⊸ B) ⊕ (G ⊸ S)}) (S ⊕ R).
+  intro p. one_step p.
+
+  apply aux6'. assumption.
+  apply aux26. assumption.
+  
+  apply aux24s. assumption.
+Qed.
+
+Hint Resolve aux23 aux25 aux6'' aux6'  aux26 aux24s aux24.
+
+Lemma aux1 : all_proofs_of ({(B ⊸ S) & (B ⊸ R), G, (G ⊸ B) ⊕ (G ⊸ S)}) (S ⊕ R).
+  intros p; one_step p.
+Qed.
+Lemma aux27r : no_proof_for ({G ⊸ S, G, ((B ⊸ S) & (B ⊸ R)) & 1}) R.
+  intros p; one_step p.
+Qed.  
+
+Lemma aux31 : no_proof_for ({G, ((B ⊸ S) & (B ⊸ R)) & 1, (G ⊸ B) ⊕ (G ⊸ S)}) R.
+  intros p.
+  one_step p.
+  apply aux27r. assumption.
+Qed.
+
+
+Lemma aux29 : no_proof_for ({(B ⊸ S) & (B ⊸ R), S}) (S ⊕ R).
+  intros p; one_step p.
+Qed.
+Lemma aux30 : all_proofs_of ({1, S}) (S ⊕ R).
+  intros p; one_step p.
+Qed.  
+Lemma aux28 : all_proofs_of ({S, ((B ⊸ S) & (B ⊸ R)) & 1}) (S ⊕ R).
+  intros p; one_step p.
+  apply False_ind. apply aux29. assumption.
+  apply aux30.
+Qed.
+
+Hint Resolve aux27r aux31 aux29 aux30 aux28.
+
+Lemma aux32 : no_proof_for ({(B ⊸ S) & (B ⊸ R), G ⊸ S, G}) (S ⊕ R).
+  intros p; one_step p.
+Qed.
+
+Lemma aux34 : all_proofs_of ({G ⊸ S, G}) (S ⊕ R).
+  intros p;one_step p.
+Qed.
+
+Lemma aux33 : all_proofs_of ({1, G ⊸ S, G}) (S ⊕ R).
+  intros p; one_step p.
+  apply aux34.
+Qed.
+
+Lemma aux27 : all_proofs_of ({G ⊸ S, G, ((B ⊸ S) & (B ⊸ R)) & 1}) (S ⊕ R).
+  intros p; one_step p.
+  apply False_ind. apply aux32. assumption.
+  apply aux33.
+Qed.
+
+Hint Resolve aux34 aux33 aux27.
+
+Lemma final: all_proofs_of ({ G,((B⊸S)&(B⊸R))&1,(G⊸B)⊕(G⊸S)}) (S⊕R).
+Proof.
+  intros p; one_step p.
+
+  apply aux1. 
+
+  rewrite aux27.
+  destruct (exist right_choices_between_S_and_R i0);reflexivity.  
+Qed.
+
