boolP.v
@@ -1,0 +1,26 @@
+Inductive boolP : Prop := trueP | falseP.
+
+Definition eq_boolP a b := 
+  match a,b with
+    | trueP,trueP => trueP
+    | falseP,falseP => trueP
+    | _,_ => falseP
+  end.
+
+Infix "?=" := eq_boolP (at level 80).
+
+Definition orP a b :=
+  match a with
+    | trueP => trueP
+    | falseP => b
+  end.
+
+
+Definition andP a b :=
+  match a with
+    | falseP => falseP
+    | trueP => b
+  end.
+
+Infix "ORP" := orP (at level 70).
+Infix "ANDP" := andP (at level 70).
